**Notation** Given integers $a$ and $b$, not both zero, we write $\gcd(a, b)$ or $(a, b)$ for the greatest common divisor of $a$ and $b$. 

>[!note] Example 1.1.1
>Very inefficiently - the positive divisors of 12 are 1, 2, 3, 4, 6 and 12, so $\gcd(12, 20)$ = 4

Is there a more efficient way to do this? 
>[!note] Example 1.1.2
>Suppose we want to find $\gcd(2024, 70)$. We have
>$$
>\begin{align}
>2024 &= 28 \times 70 + 64 \\
>70 &= 64 + 6 \\
>64 &= 10 \times 6 + 4 \\
>6 &= 4 + 2 \\
>4 &= 2 \times 2
>
>\end{align}
>$$
>So the GCD is 2.

## Euclid's Algorithm Process
We may assume that $0 < a \le b$ since $(0, b) = b$
1. Put $a_{0}= a$ and $b_{0}= b$
2. Use the division algorithm to find $q_{0}, r_{0}\in \mathbb{Z}$ such that $b_{0}= q_0a_{0}+ r_0$ and $0 \le r_{0}< a_0$
3. If $r_{0}= 0$ then $\gcd(a, b) = a_0$
4. If $0 < r_{0}< a_0$, then set $a_{1}= r_0$ and $b_{1}= a_0$, and repeat the process 

>[!note]- Proof 
>The $a_{i}\in \mathbb{Z}_{\ge 0}$ are decreasing, so the algorithm must terminate. If $b = aq + r$, then the common divisors of $r$ and $a$ are the same as the common divisors of $a$ and $b$, so $\gcd(r, a) = \gcd(a, b)$. If the algorithm terminates are $i + 1$ steps, then 
>$$a_{i}= \gcd(0, a_{i}) = \gcd(a_{i},a_{i-1}) = ... = \gcd(a_{1}, a_{0)} = \gcd(a, b)$$

--- 
>[!note] Example 1.1.3
>Euclid's algorithm can be run backwards to express the GCD as a linear combination of the two numbers. This is called the *extended Euclidean algorithm*
>We have 
>$$
>\begin{align} 
>2 &= 6 - 4 \\
>&= 6 - (64 - 10 \times 6) = 11 \times 6 - 64 \\
>&= 11(70 - 644) - 64 = 11 \times 70 - 12 \times 64 \\
>&= 11 \times 70 - 12(2024 - 28 \times 70) = 347 \times 70 - 12 \times 2024
>\end{align}
>$$
>This gives a practical way to establish the fundamental result below 

>[!multi-column]
>>[!warning] Lemma 1.1.4 (Bezout's Lemma)
>>
>>Let $a$ and $b$ be integers, not both zero. Then there exist $x, y \in \mathbb{Z}$ such that
>>$$ax + by = \gcd(a, b)$$ 
>>^bezouts
>
>>[!warning] Corollary 1.15
>>
>>Let $a$ and $b$ be integers, not both zero, and let $d \in \mathbb{Z}$. Then $d$ divides $a$ and $b$ if and only if $d \mid \gcd(a, b)$
>>>[!note]- Proof
>>>
>>>If $d$ divides $\gcd(a, b)$, then it divides $a$ and $b$. Conversely, suppose $d$ divides $a$ and $b$. For some $x, y \in \mathbb{Z}$, we have 
>>>$$\gcd(a, b) = ax + by$$
>>>which is divisible by $d$.


