Let $m \in \mathbb{N}$ We say that $0, 1,..., m-1$ form a *complete set of residues* module $m$, because they have exactly one representative from each [[1.4 Congruences#^68d73a|congruence class]]. The ring $\mathbb{Z}/m\mathbb{Z}$ is $\{0, 1, ..., m - 1\}$ equipped with addition and multiplication modulo $m$. It is easy to check that this ring is commutative.

>[!note] Example 1.5.1 (Associativity)
>Let $a, b, c \in \{0,1,..., m-1\}$. We write 
>$$ab = q_1m + r_1, \qquad bc = q_2m+r_2$$ 
>with $0 \le r_1, r_2 < m$. Then 
>$$r_1 c \equiv abc \equiv ar_2 \mod m$$ 
>hence $(ab)c = a(bc) \in \mathbb{Z}/m\mathbb{Z}$ 

**Notation** We will denote the multiplicative group of units (invertible elements) modulo $m$ by ($\mathbb{Z}/m\mathbb{Z})^{\times}$ 

>[!warning] Lemma 1.5.2
>Let $m \in \mathbb{N}$ and $a \in \mathbb{Z}$ Then $a$ is invertible modulo $m$ if and only if $\gcd(a, m) = 1$. 
>>[!note] Example 1.5.3 
>>
>>We have $(\mathbb{Z}/m\mathbb{Z})^{\times} = \{1, 5\} \mod 6$ 
>
>>[!note]- Proof
>>
>>The integer $a$ is invertible module $m$ if and only if there exist $x, y \in \mathbb{Z}$ such that $ax + my = 1$. By [[1.1 Euclid's Algorithm#^bezouts|Bezout's lemma]], such integers exist if $(a, m) = 1$, and conversely if such integers exist then $a, m$ must be coprime.

Hence $(\mathbb{Z}/m\mathbb{Z})^{\times}$ comprises the [[1.2 The Fundamental Theorem of Arithmetic#^a1320f|coprime]] residue classes modulo $m$. The *Euler totient function $\varphi$* counts the number of coprime residue classes: 
$$\varphi(m) = \#\{a \in \{1, 2, ..., \} : \gcd(a, m) = 1\}$$ Therefore $|(\mathbb{Z}/m\mathbb{Z})^{\times}| = \varphi(m)$  ^034bbc

>[!note] Example 1.5.4 
>We have $\varphi(6) = 2$

>[!Warning] Lemma 1.5.5 
>If $p$ is prime, then $\mathbb{Z}/p\mathbb{Z}$ is a field, and 
>$$(\mathbb{Z}/p\mathbb{Z})^{\times} = \{1, 2,..., p - 1\} \mod p$$ 
>has order $\varphi(p) = p - 1$ 
>>[!note]- Proof
>>
>>It is a commutative ring, and any non-zero element is invertible (being [[1.2 The Fundamental Theorem of Arithmetic#^a1320f|coprime]] to the modulus)
>
>We also denote this by $\mathbb{F}_p$. Note that if $m$ is composite then $\mathbb{Z}/m\mathbb{Z}$ isn't a field since any prime divisor of $m$ is non-invertible. 

>[!note] Example 1.5.6 
>We have 
>$$1^2 \equiv 2 \times 4 \equiv 3 \times 5 \equiv 6^2 \equiv 1 \mod 7$$ 


**Mod 13 (Card Game)** 
1. Each player is dealt a hand of cards, interpreted as residue classes modulo 13, and two cards $a_1, a_2$ are placed into the centre. 
2. Racing, a player can either play the sum ($a_1 + a_2), product ($a_1a_2$), arithmetic progression ($2a_2 - a_1$) or geometric progression ($a_2^2a_1^{-1}$) as the card $a_3$, declaring what type of move they have made 
3. Play continues with cards $a_2$ and $a_3$ in place of $a_1$ and $a_2$ and so on, until somebody finishes and wins 

>[!note] Example 1.5.7 
>Geometric progression: 7, J, and..? We have 
>$$11 \equiv 24 \equiv 4(-7) \equiv 9 \times 7 \mod 13$$
>so the next card is 
>$$9 \times 11 \equiv 8$$

>[!warning] Lemma 1.5.8 (Solving a linear congruence)
>Let $a, b \in \mathbb{Z}$ and $m \in \mathbb{N}$. Then: #
>(a) There exists $a \in \mathbb{Z}$ solving $ax \equiv b\mod m$ if and only if $\gcd(a, m) \mid b$ 
>(b) If $\gcd(a, m) \mid b$ and $x_0 \in \mathbb{Z}$ is a solution to $ax_0 \equiv b \mod m$, then all solutions are given by 
>$$ x_0 + \frac{tm}{\gcd(a, m)} \qquad (t \in \mathbb{Z})$$
>
>>[!note]- Proof
>>
>>Put 
>>$$g = \gcd(a, m), \quad a = ga', \quad m = gm'$$ 
>>so that $(a', m') = 1$
>>(a) if $x \in \mathbb{Z}$ and $ax \equiv b \mod m$ then $b \equiv ax \equiv 0 \mod g$. Conversely, if $g \mid b$ then, writing $b = gb'$, our congruence becomes $a'x \equiv b' \mod m'$. This has a solution because $(a', m') = 1$. It's given by $b'$ times the inverse of $a'$ module $m'$. 
>>(b) If $t \in \mathbb{Z}$ and $x = x_0 + tm/g$ then $ax \equiv b + atm/g \equiv b \mod m$. It remains to show that there are no other solutions. If $x$ solves the congruence then $a'x \equiv b' \equiv a'x_0 \mod m'$, so $m'$ divides $x - x_0$ by the [[1.2 The Fundamental Theorem of Arithmetic#^8a00b4|general Euclid lemma]]. Therefore $x = X_0 + tm'$ for some $t \in \mathbb{Z}$.
>>

>[!warning] Theorem 1.5.10 (Classical Chinese Remainder Theorem)
>Let $m_1,...m_K \in \mathbb{N}$ be pairwise [[1.2 The Fundamental Theorem of Arithmetic#^a1320f|coprime]], and let $a_1, ..., a_K \in \mathbb{Z}$. Then there exists $x \in \mathbb{Z}$, unique modulo $\prod_k m_k$ such that 
>$$x \equiv a_k \mod m_k \quad (1 \le k \le K)$$ 
>This is given by $\sum_i a_i M_i y_i$, where $M_i = \prod_{j \ne i} m_j$ and $M_i y_i \equiv 1 \mod m_i$
>
>>[!note]- Proof
>>For existence, observe that for each $k$ we have 
>>$$\sum_i a_i M_i y_i \equiv a_k M_k y_k \equiv a_k \mod m_k$$
>>For uniqueness, observe that if $x, y$ are solutions then $x - y$ is divisible by $m_1,..., m_K$. As the $m_i$ are pairwise coprime, it follows from [[1.2 The Fundamental Theorem of Arithmetic#^ftoa|the fundamental theorem of arithmetic]] that $m_1...m_K$ divides $x - y$

>[!warning] Theorem 1.5.14 (Algebraic Chinese Remainder Theorem)
>Let $m_1,...,m_K \in \mathbb{N}$ be pairwise [[1.2 The Fundamental Theorem of Arithmetic#^a1320f|coprime]], and put $M = \prod_k m_k$. Then 
>$$\psi : \mathbb{Z}/M\mathbb{Z} \to \mathbb{Z}/m_1 \mathbb{Z} \times ... \times \mathbb{Z}/m_K\mathbb{Z}$$ 
>$$x \mapsto (x \mod m_1,..., x \mod m_K)$$
>is a ring isomorphism. Moreover, it restricts to a group isomorphism
>$$(\mathbb{Z}/M\mathbb{Z})^{\times} \to (\mathbb{Z}/m_1\mathbb{Z})^{\times} \times ... \times (\mathbb{Z}/m_k\mathbb{Z})^{\times}$$
>>[!note]- Proof
>>
>>Well-defined: If $x \in \mathbb{Z}$ then 
>>$$x + M \equiv x \mod m_k \quad (1 \le k \le K)$$ 
>>We saw that modular arithmetic [[1.4 Congruences#^0fedf7|respects addition and multiplication]], so $\psi$ is a ring homomorphism. The classical Chinese remainder theorem defines an inverse function, so $\psi$ is bijective and therefore an isomorphism. 
>>For the second part, note that $x \in \mathbb{Z}/M\mathbb{Z}$ is [[1.2 The Fundamental Theorem of Arithmetic#^a1320f|coprime]] to $M$ if and only if it's coprime to each $m_k$. Therefore $\psi$ restricts to a bijection 
>>$$(\mathbb{Z}/M\mathbb{Z})^{\times} \to (\mathbb{Z}/ m_1 \mathbb{Z})^{\times} \times ... \times (\mathbb{Z}/m_k\mathbb{Z})^{\times}$$
>>This is a group homomorphism because $\psi$ is a ring homomorphism. Hence, it's a group isomorphism. 

Recall that an [[1.3 Fermat Primes, Mersenne Primes, and Perfect Numbers#^44ecc6|arithmetic function]] is a function $\mathbb{N} \to \mathbb{C}$ and than an arithmetic function $f$ is *multiplicative* if $f(mn) = f(m) f(n)$ holds for any [[1.2 The Fundamental Theorem of Arithmetic#^a1320f|coprime]] positive integers $m$ and $n$. 

>[!warning] Corollary 1.5.15
>[[1.5 Linear Congruences#^034bbc|Euler's totient function]] is multiplicative
>>[!note]- Proof 
>>
>>Apply the algebraic Chinese remainder theorem with $K = 2$

>[!warning] Lemma 1.5.16
>For $n \in \mathbb{N}$ we have 
>$$\varphi(n) = n \prod_{p \mid n} (1 - \frac{1}{p})$$ 
>where the product is over primes dividing $n$. 
>>[!note]- Proof 
>>
>>Observe that $\varphi(1) = 1$. Next, suppose $n = p^k$ for some prime $p$ and some $k \in \mathbb{N}$. then $\varphi(n)$ is he number of residue classes that aren't divisible by $p$, which is 
>>$$p^k - p^{k - 1} = p^k (1 - \frac{1}{p})$$
>>Finally, suppose $n = p_1^{k_1}...p_r^{k_r}$, where the $p_i$ are pairwise distinct primes and the $k_i$ are positive integers. Then 
>>$$\varphi(n) = \prod_{i \le r} \varphi(p^{k_i}) = \prod_{i \le r} p^{k_i} (1 - \frac{1}{p}) = n \prod_{p \mid n} (1 - \frac{1}{p})$$

>[!warning] Lemma 1.5.18 (Totient function identity)
>For $n \in \mathbb{N}$, we have 
>$$\sum_{d \mid n} \varphi(d) = n$$ 
>where the sum is over the positive divisors of $n$
>>[!note]- Proof 
>>
>>There are 2 steps to this proof:
>>First, we show that the arithmetic function 
>>$$f(n) = \sum_{d \mid n} \varphi(d)$$ 
>>is multiplicative. Let $m$ and $n$ be [[1.2 The Fundamental Theorem of Arithmetic#^a1320f|coprime]] positive integers. Then the positive divisors of $m$ are the numbers of the form $de$, where $d, e$ are positive divisors of $m, n$ respectively, and $(d, e) = 1$. This 
>>$$f(mn) = \sum_{d \mid m} \sum_{e \mid n} \varphi(de) = \sum_{d \mid m} \sum_{e \mid n} \varphi(d)\varphi(e) = f(m)f(n)$$ 
>>So $f$ is multiplicative. 
>>It remains to prove that $f(p^k) = p^k$ for any prime power $p^k$. We compute:
>>$$f(p^k) = \sum_{j = 1}^{k} \varphi(p^j) = 1 + (p - 1) + (p^2 - p) + ... + (p^k - p^{k - 1}) = p^k$$ 

